finalised for submission

Assignment1/Ex7.dfy
@@ -5,10 +5,6 @@
 //                 September 2019                          //
 /////////////////////////////////////////////////////////////
 
-// functions were used to allow for my specification to have 
-// functional behaviour e.g. counting
-// link to resource: https://www.engr.mun.ca/~theo/Courses/AlgCoCo/6892-downloads/dafny-notes-010.pdf
-
 // Ex7.dfy 10 marks. 
 // Write a Dafny method Just1;
 // This method should return true if and only if the array contains just one instance of the key. 
@@ -32,56 +28,41 @@
 
 method Just1(a: array<int>, key: int) returns (b: bool)
 requires a != null
-ensures b == (CountOccurences(a, key, a.Length - 1) == 1)
+ensures b == (CountOccurences(a[0..a.Length], key) == 1)
 ensures forall i :: 0 <= i < a.Length ==> (a[i] == old(a[i]))
 {
-
+    // note we did not do an initial assumption like Ex6
+    // since we are tackling a different problem
     var i := 0;
     var count := 0;
     while i < a.Length
     invariant 0 <= i <= a.Length
-    invariant count == CountOccurences(a, key, i-1)
+    // this invariant says that our running counter
+    // should match the number of occurences
+    // found in a multiset created from the sequence a
+    // up until the index i
+    invariant count == CountOccurences(a[0..i], key)
     {
+        // if we encounter a key increment our counter by 1
         if(a[i] == key)
         {
             count := count + 1;
         }
         i := i + 1;
     }
+    // so now we just return the statement that 
+    // count == 1
     b := (count == 1);
 }
 
-// this function will be used to count the number of occurences of the key
-// in the array a, up until the index provided
-function CountOccurences(a: array<int>, key: int, index: int): int
-requires a != null
-requires index < a.Length
-// short circuit checking first :), this is only really here just so 
-// i can perform my assertions on occurences in array, no functional reason
-ensures (index < 0) ==> (CountOccurences(a, key, index) == 0)
-ensures (index >= 0 && a[index] == key) ==> (CountOccurences(a, key, index) == 1 + CountOccurences(a, key, index - 1))
-ensures (index >= 0 && a[index] != key) ==> (CountOccurences(a, key, index) ==  CountOccurences(a, key, index - 1))
-reads a
-// here i supply my variant that maxIndex is decreasing
-decreases index
+// this function will take in a sequence and 
+// create a multi-set from the sequence
+// it will then return the occurences of the key within
+// the multiset, all handled by the good old duck Dafny
+function CountOccurences(a: seq<int>, key: int): int 
+ensures CountOccurences(a, key) == multiset(a)[key]
 {
-    if index < 0 
-    then
-        0
-    else
-        if a[index] == key 
-        then
-            CountOccurences(a, key, index - 1) + 1
-        else
-            CountOccurences(a, key, index - 1) 
-}
-
-predicate VerifyJustOne(a: array<int>, key: int)
-requires a != null;
-reads a;
-{
-    (exists i :: 0 <= i < a.Length && a[i] == key) &&
-    (forall i,j :: 0 <= i <= j < a.Length && (a[i] == a[j]) && (a[i] == key) ==> i == j)
+    multiset(a)[key]
 }
 
 method Main()
@@ -97,50 +78,37 @@ method Main()
     assert testArray1[1] == 1;
     assert testArray1[2] == 2;
     assert testArray1[3] == 1;
-    var test1 := Just1(testArray1, 1);
-    assert (CountOccurences(testArray1, 1, testArray1.Length - 1) == 3);
-    assert !VerifyJustOne(testArray1, 1);
-    assert !test1;
-
-    assert testArray1.Length == 4;
-    assert testArray1[0] == 1;
-    assert testArray1[1] == 1;
-    assert testArray1[2] == 2;
-    assert testArray1[3] == 1;
-    var test2 := Just1(testArray1, 2);
-    assert (CountOccurences(testArray1, 2, testArray1.Length - 1) == 1);
-    assert VerifyJustOne(testArray1, 2);
-    assert test2;
-    
-    assert testArray1.Length == 4;
-    assert testArray1[0] == 1;
-    assert testArray1[1] == 1;
-    assert testArray1[2] == 2;
-    assert testArray1[3] == 1;
-    var test3 := Just1(testArray1, 3);
-    assert (CountOccurences(testArray1, 3, testArray1.Length - 1) == 0);
-    assert !VerifyJustOne(testArray1, 3);
-    assert !test3;
 
     assert testArray2.Length == 1;
     assert testArray2[0] == 1;
-    var test4 := Just1(testArray2, 1);
-    assert (CountOccurences(testArray2, 1, testArray2.Length - 1) == 1);
-    assert VerifyJustOne(testArray2, 1);
-    assert test4;
-
-    assert testArray2.Length == 1;
-    assert testArray2[0] == 1;
-    var test5 := Just1(testArray2, 2);
-    assert (CountOccurences(testArray2, 2, testArray2.Length - 1) == 0);
-    assert !VerifyJustOne(testArray2, 2);
-    assert !test5;
 
     assert testArray3.Length == 0;
+
+    var test1 := Just1(testArray1, 1);
+    assert CountOccurences(testArray1[0..testArray1.Length], 1) == 3;
+    assert !test1;
+
+
+    var test2 := Just1(testArray1, 2);
+    assert CountOccurences(testArray1[0..testArray1.Length], 2) == 1;
+    assert test2;
+    
+    var test3 := Just1(testArray1, 3);
+    assert CountOccurences(testArray1[0..testArray1.Length], 3) == 0;
+    assert !test3;
+
+    var test4 := Just1(testArray2, 1);
+    assert CountOccurences(testArray2[0..testArray2.Length], 1) == 1;
+    assert test4;
+
+    var test5 := Just1(testArray2, 2);
+    assert CountOccurences(testArray2[0..testArray2.Length], 2) == 0;
+    assert !test5;
+
     var test6 := Just1(testArray3, 1);
-    assert (CountOccurences(testArray3, 1, testArray3.Length - 1) == 0);
-    assert !VerifyJustOne(testArray3, 1);
+    assert CountOccurences(testArray3[0..testArray3.Length], 1) == 0;
     assert !test6;
 
     print test1, "\n", test2, "\n", test3, "\n", test4, "\n", test5, "\n", test6, "\n";
+
 }
