Assignment1/Ex7a.dfy
@@ -32,14 +32,15 @@
 
 method Just1(a: array<int>, key: int) returns (b: bool)
 requires a != null
-ensures b == (counte(a[0..a.Length], key) == 1)
+ensures b == (CountOccurences(a, key, a.Length - 1) == 1)
 ensures forall i :: 0 <= i < a.Length ==> (a[i] == old(a[i]))
 {
+
     var i := 0;
     var count := 0;
     while i < a.Length
     invariant 0 <= i <= a.Length
-    invariant count == counte(a[0..i], key)
+    invariant count == CountOccurences(a, key, i-1)
     {
         if(a[i] == key)
         {
@@ -50,10 +51,37 @@ ensures forall i :: 0 <= i < a.Length ==> (a[i] == old(a[i]))
     b := (count == 1);
 }
 
-function counte(a: seq<int>, key: int): int 
-ensures counte(a, key) == multiset(a)[key]
+// this function will be used to count the number of occurences of the key
+// in the array a, up until the index provided
+function CountOccurences(a: array<int>, key: int, index: int): int
+requires a != null
+requires index < a.Length
+// short circuit checking first :), this is only really here just so 
+// i can perform my assertions on occurences in array, no functional reason
+ensures (index < 0) ==> (CountOccurences(a, key, index) == 0)
+ensures (index >= 0 && a[index] == key) ==> (CountOccurences(a, key, index) == 1 + CountOccurences(a, key, index - 1))
+ensures (index >= 0 && a[index] != key) ==> (CountOccurences(a, key, index) ==  CountOccurences(a, key, index - 1))
+reads a
+// here i supply my variant that maxIndex is decreasing
+decreases index
 {
-    multiset(a)[key]
+    if index < 0 
+    then
+        0
+    else
+        if a[index] == key 
+        then
+            CountOccurences(a, key, index - 1) + 1
+        else
+            CountOccurences(a, key, index - 1) 
+}
+
+predicate VerifyJustOne(a: array<int>, key: int)
+requires a != null;
+reads a;
+{
+    (exists i :: 0 <= i < a.Length && a[i] == key) &&
+    (forall i,j :: 0 <= i <= j < a.Length && (a[i] == a[j]) && (a[i] == key) ==> i == j)
 }
 
 method Main()
@@ -69,37 +97,50 @@ method Main()
     assert testArray1[1] == 1;
     assert testArray1[2] == 2;
     assert testArray1[3] == 1;
+    var test1 := Just1(testArray1, 1);
+    assert (CountOccurences(testArray1, 1, testArray1.Length - 1) == 3);
+    assert !VerifyJustOne(testArray1, 1);
+    assert !test1;
+
+    assert testArray1.Length == 4;
+    assert testArray1[0] == 1;
+    assert testArray1[1] == 1;
+    assert testArray1[2] == 2;
+    assert testArray1[3] == 1;
+    var test2 := Just1(testArray1, 2);
+    assert (CountOccurences(testArray1, 2, testArray1.Length - 1) == 1);
+    assert VerifyJustOne(testArray1, 2);
+    assert test2;
+    
+    assert testArray1.Length == 4;
+    assert testArray1[0] == 1;
+    assert testArray1[1] == 1;
+    assert testArray1[2] == 2;
+    assert testArray1[3] == 1;
+    var test3 := Just1(testArray1, 3);
+    assert (CountOccurences(testArray1, 3, testArray1.Length - 1) == 0);
+    assert !VerifyJustOne(testArray1, 3);
+    assert !test3;
 
     assert testArray2.Length == 1;
     assert testArray2[0] == 1;
-
-    assert testArray3.Length == 0;
-
-    var test1 := Just1(testArray1, 1);
-    assert counte(testArray1[0..testArray1.Length], 1) == 3;
-    assert !test1;
-
-
-    var test2 := Just1(testArray1, 2);
-    assert counte(testArray1[0..testArray1.Length], 2) == 1;
-    assert test2;
-    
-    var test3 := Just1(testArray1, 3);
-    assert counte(testArray1[0..testArray1.Length], 3) == 0;
-    assert !test3;
-
     var test4 := Just1(testArray2, 1);
-    assert counte(testArray2[0..testArray2.Length], 1) == 1;
+    assert (CountOccurences(testArray2, 1, testArray2.Length - 1) == 1);
+    assert VerifyJustOne(testArray2, 1);
     assert test4;
 
+    assert testArray2.Length == 1;
+    assert testArray2[0] == 1;
     var test5 := Just1(testArray2, 2);
-    assert counte(testArray2[0..testArray2.Length], 2) == 0;
+    assert (CountOccurences(testArray2, 2, testArray2.Length - 1) == 0);
+    assert !VerifyJustOne(testArray2, 2);
     assert !test5;
 
+    assert testArray3.Length == 0;
     var test6 := Just1(testArray3, 1);
-    assert counte(testArray3[0..testArray3.Length], 1) == 0;
+    assert (CountOccurences(testArray3, 1, testArray3.Length - 1) == 0);
+    assert !VerifyJustOne(testArray3, 1);
     assert !test6;
 
     print test1, "\n", test2, "\n", test3, "\n", test4, "\n", test5, "\n", test6, "\n";
-
 }
