Assignment1/Ex2.dfy
@@ -10,6 +10,10 @@
 // Verify in Dafny that every integer is either even or odd.
 
 method main(number:int){
+    // the parity of a number is it's remainder when divided by 2
+    // parity == 1 means the number is odd
+    // parity == 0 means the number is even
     var parity := number%2;
+    // the assert states that the parity is either 0 or 1, verifying the statement
     assert parity == 0 || parity == 1;
 }
