Assignment1/Ex3.dfy
@@ -17,9 +17,15 @@ var skip := 7;
 var index := 0;
 
 while index<=limit
+// pred 1 
 invariant index <= limit + skip
 invariant index == ((index/skip))*skip
-{ index := index+skip; }
+// end pred 1
+{
+     index := index+skip; 
+}
+// pred 2
 assert index >= limit;
 assert index == ((index/skip))*skip;
+// end pred 2
 }
